Corrections

2016/Lambda_calculus.thy
@@ -110,8 +110,7 @@ function subst_L :: "nat \<Rightarrow> lterm \<Rightarrow> lterm \<Rightarrow> l
   "subst_L j s (Seq t1 t2) = Seq (subst_L j s t1) (subst_L j s t2)" |
   "subst_L j s (t as A) = (subst_L j s t) as A" |
   "subst_L j s (Let var x := t in t1) = 
-  (if j=x then Let var x := subst_L j s t in t1
-    else  (Let var x := (subst_L j s t) in (subst_L (if j > x then Suc j else j) (if j > x then (shift_L 1 x s) else s) t1))) " |
+  ((Let var x := (subst_L j s t) in (subst_L (if j \<ge> x then Suc j else j) (shift_L 1 x s) t1))) " |
   "subst_L j s (\<lbrace>t1,t2\<rbrace>) = \<lbrace>subst_L j s t1, subst_L j s t2\<rbrace>" |
   "subst_L j s (\<pi>1 t) = \<pi>1 (subst_L j s t)" |
   "subst_L j s (\<pi>2 t) = \<pi>2 (subst_L j s t)" |
@@ -125,11 +124,11 @@ function subst_L :: "nat \<Rightarrow> lterm \<Rightarrow> lterm \<Rightarrow> l
   "subst_L j s (inr t as T') =  inr (subst_L j s t) as T'" |
   "subst_L j s (Case t of Inl x \<Rightarrow> t1 | Inr y \<Rightarrow> t2) = 
     (Case (subst_L j s t) of 
-        Inl x \<Rightarrow> (if j=x then t1 else subst_L (if j > x then Suc j else j) (shift_L 1 x s) t1)
-      | Inr y \<Rightarrow> (if j=y then t2 else subst_L (if j > y then Suc j else j) (shift_L 1 y s) t2))" |
+        Inl x \<Rightarrow> (subst_L (if j \<ge> x then Suc j else j) (shift_L 1 x s) t1)
+      | Inr y \<Rightarrow> (subst_L (if j \<ge> y then Suc j else j) (shift_L 1 y s) t2))" |
   "subst_L j s (<l:=t> as T') =  <l:=subst_L j s t> as T'" |
   "subst_L j s (Case t of <L:=I> \<Rightarrow> LT) = 
-    (Case (subst_L j s t) of <L:=I> \<Rightarrow> map (\<lambda>p. if j=fst p then snd p else subst_L (if j > fst p  then Suc j else j) (shift_L 1 (fst p) s) (snd p)) (zip I LT))" |
+    (Case (subst_L j s t) of <L:=I> \<Rightarrow> map (\<lambda>p. subst_L (if j \<ge> fst p  then Suc j else j) (shift_L 1 (fst p) s) (snd p)) (zip I LT))" |
   "subst_L j s (Fixpoint t) = Fixpoint (subst_L j s t)"|
   "subst_L j s (Lnil A) = Lnil A"|
   "subst_L j s (Lisnil A t) = Lisnil A (subst_L j s t)"|
@@ -142,14 +141,7 @@ termination
   by (relation "measure (\<lambda>(j,s,t). size t)", simp_all)
       (metis less_add_Suc1 size_list_estimation' set_zip_rightD 
               lessI not_less prod.collapse)+
-  
-text{*
-      We want to restrict the considered pattern matching and filling to coherent cases, which are
-      the cases when a pattern variable can only appear once in a given pattern.\\
 
-      Furthermore, the same coherence principle is valid for the pattern context. A pattern variable can only 
-      have on type at a time
-*}
 
 fun Pvars :: "Lpattern \<Rightarrow> nat list" where
 "Pvars (V n as A) = [n]" |
@@ -238,19 +230,6 @@ termination
       (metis less_add_Suc1 size_list_estimation' set_zip_rightD 
               lessI not_less prod.collapse)+
 
-text{*
-    We implement pattern matching and replacing with the following function and definition:
-    
-    \begin{itemize}
-      \item a \textbf{pattern context} 
-      \item a \textbf{pattern substitution} is a list of pairs (pattern var index, lterm)
-      \item \textbf{fill}, which will fill the patterns in a ltern with a lterm (based on a pattern substitution)
-      \item \textbf{Lmatch} is a predicate on a pattern, a value and a pattern substitution indicating 
-              if the pattern substitution associates the given pattern's variables to the corresponding part(s) of the
-              given value
-    \end{itemize}
-*}
-
 
 fun p_instantiate::"(nat \<rightharpoonup> lterm) \<Rightarrow> Lpattern \<Rightarrow> lterm" where
 "p_instantiate \<Sigma> (V k as A) = (case \<Sigma> k of Some t' \<Rightarrow> t' | None \<Rightarrow> <|V k as A|>)"|
@@ -310,29 +289,6 @@ fun subterms :: "lterm\<Rightarrow>subterm_set" where
 "subterms (Ltail A t)                  = Unary t" |
 "subterms (Lisnil A t)                  = Unary t" |
 "subterms t = Void"
-
-lemma P_list_conv_nth:"(\<And>x. x\<in> A\<union>set L \<Longrightarrow> P x) \<Longrightarrow> (\<And>i. i<length L \<Longrightarrow> P (L!i))"
-using set_conv_nth by auto
-
-lemma P_pat_subterm_cases:
-  "P (patterns t) \<Longrightarrow> (\<exists>t1. subterms t = Unary t1 \<and> P (patterns t1)) \<or>
-    (\<exists>t1 t2. subterms t = Bi t1 t2 \<and> P (patterns t1) \<and> P (patterns t2)) \<or>
-    (\<exists>t1 t2 t3. subterms t = Ter t1 t2 t3 \<and> P (patterns t1) \<and> P (patterns t2) \<and> P (patterns t3)) \<or>
-    (\<exists>t1 L. subterms t = Comp t1 L \<and> P (patterns t1) \<and> (\<forall>i<length L. P (patterns (L!i)))) \<or>
-    (\<exists>L. subterms t = UList L \<and> (\<forall>i<length L. P (patterns (L!i))))" 
-sorry
-
-ML \<open>
-      fun rewrite_conj_under_all ctxt thm = 
-        (case ctxt of
-          Context.Theory _ => thm
-          |Context.Proof prf =>
-              thm
-              |> Local_Defs.unfold prf [@{thm atomize_conj[symmetric]}, @{thm atomize_all[symmetric]}, 
-                                          @{thm atomize_imp[symmetric]}]
-        )
-   \<close>
-attribute_setup split_and_rule = \<open>Scan.succeed (Thm.rule_attribute [] rewrite_conj_under_all)\<close>
 
 
 end
